<?xml version="1.0"?>
<rdf:RDF xmlns="http://www.dmi.unict.it/ec-oasis.owl#"
     xml:base="http://www.dmi.unict.it/ec-oasis.owl"
     xmlns:owl="http://www.w3.org/2002/07/owl#"
     xmlns:rdf="http://www.w3.org/1999/02/22-rdf-syntax-ns#"
     xmlns:xml="http://www.w3.org/XML/1998/namespace"
     xmlns:xsd="http://www.w3.org/2001/XMLSchema#"
     xmlns:rdfs="http://www.w3.org/2000/01/rdf-schema#"
     xmlns:oasis="http://www.dmi.unict.it/oasis.owl#"
     xmlns:terms="http://purl.org/dc/terms/">
    <owl:Ontology rdf:about="http://www.dmi.unict.it/ec-oasis.owl">
        <owl:imports rdf:resource="http://www.dmi.unict.it/oasis-abox.owl"/>
        <owl:imports rdf:resource="http://www.dmi.unict.it/oasis.owl"/>
    </owl:Ontology>
    


    <!-- 
    ///////////////////////////////////////////////////////////////////////////////////////
    //
    // Object Properties
    //
    ///////////////////////////////////////////////////////////////////////////////////////
     -->

    


    <!-- http://www.dmi.unict.it/ec-oasis.owl#hasAcquisitionFee -->

    <owl:ObjectProperty rdf:about="http://www.dmi.unict.it/ec-oasis.owl#hasAcquisitionFee">
        <rdfs:subPropertyOf rdf:resource="http://www.dmi.unict.it/ec-oasis.owl#hasFee"/>
        <rdfs:domain rdf:resource="http://www.dmi.unict.it/ec-oasis.owl#SupplyChainAcquisitionPlan"/>
        <rdfs:range rdf:resource="http://www.dmi.unict.it/ec-oasis.owl#Fee"/>
        <rdfs:comment xml:lang="eng">This property connects an acquisition plan of supply chain with the related fee costs</rdfs:comment>
        <rdfs:comment xml:lang="eng">has Acquisition Fee</rdfs:comment>
    </owl:ObjectProperty>
    


    <!-- http://www.dmi.unict.it/ec-oasis.owl#hasAvailabilityPeriod -->

    <owl:ObjectProperty rdf:about="http://www.dmi.unict.it/ec-oasis.owl#hasAvailabilityPeriod">
        <rdfs:subPropertyOf rdf:resource="http://www.dmi.unict.it/ec-oasis.owl#isAvailabilityFeatureDescribedBy"/>
        <rdfs:subPropertyOf rdf:resource="http://www.dmi.unict.it/oasis.owl#hasTimeSpan"/>
        <rdfs:domain rdf:resource="http://www.dmi.unict.it/ec-oasis.owl#OfferingAvailability"/>
        <rdfs:range rdf:resource="http://www.dmi.unict.it/oasis.owl#TimeWindow"/>
        <rdfs:comment xml:lang="eng">This property connects an availability feature with the related validity window</rdfs:comment>
        <rdfs:label xml:lang="eng">has Availability Period</rdfs:label>
    </owl:ObjectProperty>
    


    <!-- http://www.dmi.unict.it/ec-oasis.owl#hasBasePrice -->

    <owl:ObjectProperty rdf:about="http://www.dmi.unict.it/ec-oasis.owl#hasBasePrice">
        <rdfs:subPropertyOf rdf:resource="http://www.dmi.unict.it/ec-oasis.owl#hasPrice"/>
        <rdfs:domain rdf:resource="http://www.dmi.unict.it/ec-oasis.owl#Auction"/>
        <rdfs:range rdf:resource="http://www.dmi.unict.it/ec-oasis.owl#AuctionBasePrice"/>
        <rdfs:comment xml:lang="eng">This property connects an auction with the related starting price</rdfs:comment>
        <rdfs:label xml:lang="eng">has Base Price</rdfs:label>
    </owl:ObjectProperty>
    


    <!-- http://www.dmi.unict.it/ec-oasis.owl#hasEligibilityLocation -->

    <owl:ObjectProperty rdf:about="http://www.dmi.unict.it/ec-oasis.owl#hasEligibilityLocation">
        <rdfs:subPropertyOf rdf:resource="http://www.dmi.unict.it/oasis.owl#hasSpaceSpan"/>
        <rdfs:domain rdf:resource="http://www.dmi.unict.it/ec-oasis.owl#LocationEligibility"/>
        <rdfs:range rdf:resource="http://www.dmi.unict.it/oasis.owl#Space"/>
        <rdfs:comment xml:lang="eng">This property connects an eligibility feature with the related physical space</rdfs:comment>
        <rdfs:label xml:lang="eng">has Eligibility Location</rdfs:label>
    </owl:ObjectProperty>
    


    <!-- http://www.dmi.unict.it/ec-oasis.owl#hasFee -->

    <owl:ObjectProperty rdf:about="http://www.dmi.unict.it/ec-oasis.owl#hasFee">
        <rdfs:subPropertyOf rdf:resource="http://www.dmi.unict.it/oasis.owl#hasCost"/>
        <rdfs:range rdf:resource="http://www.dmi.unict.it/ec-oasis.owl#Fee"/>
        <rdfs:comment xml:lang="eng">This property connects objects with the related fee costs</rdfs:comment>
        <rdfs:comment xml:lang="eng">has Fee</rdfs:comment>
    </owl:ObjectProperty>
    


    <!-- http://www.dmi.unict.it/ec-oasis.owl#hasMaxPurchasableQuantity -->

    <owl:ObjectProperty rdf:about="http://www.dmi.unict.it/ec-oasis.owl#hasMaxPurchasableQuantity">
        <rdfs:subPropertyOf rdf:resource="http://www.dmi.unict.it/ec-oasis.owl#hasPurchasableQuantity"/>
        <rdfs:domain rdf:resource="http://www.dmi.unict.it/ec-oasis.owl#OfferingAvailability"/>
        <rdfs:range rdf:resource="http://www.dmi.unict.it/oasis.owl#Quantity"/>
        <rdfs:comment xml:lang="eng">This property connects an offering with the associated maximum purchasable quantity feature</rdfs:comment>
        <rdfs:label xml:lang="eng">has Max Purchasable Quantity</rdfs:label>
    </owl:ObjectProperty>
    


    <!-- http://www.dmi.unict.it/ec-oasis.owl#hasMaxQuantityAvailable -->

    <owl:ObjectProperty rdf:about="http://www.dmi.unict.it/ec-oasis.owl#hasMaxQuantityAvailable">
        <rdfs:subPropertyOf rdf:resource="http://www.dmi.unict.it/ec-oasis.owl#hasQuantityAvailable"/>
        <rdfs:domain rdf:resource="http://www.dmi.unict.it/ec-oasis.owl#OfferingAvailability"/>
        <rdfs:range rdf:resource="http://www.dmi.unict.it/oasis.owl#Measurement"/>
        <rdfs:comment xml:lang="eng">This property connects an offering with the associated maximum quantity availability feature</rdfs:comment>
        <rdfs:label xml:lang="eng">has Max Quantity Available</rdfs:label>
    </owl:ObjectProperty>
    


    <!-- http://www.dmi.unict.it/ec-oasis.owl#hasMinPurchasableQuantity -->

    <owl:ObjectProperty rdf:about="http://www.dmi.unict.it/ec-oasis.owl#hasMinPurchasableQuantity">
        <rdfs:subPropertyOf rdf:resource="http://www.dmi.unict.it/ec-oasis.owl#hasPurchasableQuantity"/>
        <rdfs:domain rdf:resource="http://www.dmi.unict.it/ec-oasis.owl#OfferingAvailability"/>
        <rdfs:range rdf:resource="http://www.dmi.unict.it/oasis.owl#Quantity"/>
        <rdfs:comment xml:lang="eng">This property connects an offering with the associated minimum purchasable quantity feature</rdfs:comment>
        <rdfs:label xml:lang="eng">has Min Purchasable Quantity</rdfs:label>
    </owl:ObjectProperty>
    


    <!-- http://www.dmi.unict.it/ec-oasis.owl#hasNextNegotiation -->

    <owl:ObjectProperty rdf:about="http://www.dmi.unict.it/ec-oasis.owl#hasNextNegotiation">
        <rdfs:subPropertyOf rdf:resource="http://www.dmi.unict.it/oasis.owl#evolvesIn"/>
        <rdfs:domain rdf:resource="http://www.dmi.unict.it/ec-oasis.owl#NegotiationActivity"/>
        <rdfs:range rdf:resource="http://www.dmi.unict.it/ec-oasis.owl#NegotiationActivity"/>
        <rdfs:comment xml:lang="eng">This property connects a negotiation with the subsequent one</rdfs:comment>
        <rdfs:label xml:lang="eng">has Next Negotiation</rdfs:label>
    </owl:ObjectProperty>
    


    <!-- http://www.dmi.unict.it/ec-oasis.owl#hasOfferingAvailability -->

    <owl:ObjectProperty rdf:about="http://www.dmi.unict.it/ec-oasis.owl#hasOfferingAvailability">
        <rdfs:subPropertyOf rdf:resource="http://www.dmi.unict.it/oasis.owl#hasFeature"/>
        <rdfs:domain rdf:resource="http://www.dmi.unict.it/ec-oasis.owl#CommercialIssue"/>
        <rdfs:range rdf:resource="http://www.dmi.unict.it/ec-oasis.owl#OfferingAvailability"/>
        <rdfs:comment xml:lang="eng">This property connects offering the related availability</rdfs:comment>
        <rdfs:label xml:lang="eng">has Offering Availability</rdfs:label>
    </owl:ObjectProperty>
    


    <!-- http://www.dmi.unict.it/ec-oasis.owl#hasOfferingEligibility -->

    <owl:ObjectProperty rdf:about="http://www.dmi.unict.it/ec-oasis.owl#hasOfferingEligibility">
        <rdfs:subPropertyOf rdf:resource="http://www.dmi.unict.it/oasis.owl#isRelatedWith"/>
        <rdfs:domain rdf:resource="http://www.dmi.unict.it/ec-oasis.owl#Offering"/>
        <rdfs:range rdf:resource="http://www.dmi.unict.it/ec-oasis.owl#LocationEligibility"/>
        <rdfs:comment xml:lang="eng">This property connects an offering with its eligibility feature</rdfs:comment>
        <rdfs:label xml:lang="eng">has Offering Eligibility</rdfs:label>
    </owl:ObjectProperty>
    


    <!-- http://www.dmi.unict.it/ec-oasis.owl#hasOfferingPrice -->

    <owl:ObjectProperty rdf:about="http://www.dmi.unict.it/ec-oasis.owl#hasOfferingPrice">
        <rdfs:subPropertyOf rdf:resource="http://www.dmi.unict.it/ec-oasis.owl#hasPrice"/>
        <rdf:type rdf:resource="http://www.w3.org/2002/07/owl#FunctionalProperty"/>
        <rdfs:domain rdf:resource="http://www.dmi.unict.it/ec-oasis.owl#CommercialIssue"/>
        <rdfs:range rdf:resource="http://www.dmi.unict.it/ec-oasis.owl#OfferingPrice"/>
        <rdfs:comment xml:lang="eng">This property connects an offering with the associated price</rdfs:comment>
        <rdfs:label xml:lang="eng">has Offering Price</rdfs:label>
    </owl:ObjectProperty>
    


    <!-- http://www.dmi.unict.it/ec-oasis.owl#hasPaymentFee -->

    <owl:ObjectProperty rdf:about="http://www.dmi.unict.it/ec-oasis.owl#hasPaymentFee">
        <rdfs:subPropertyOf rdf:resource="http://www.dmi.unict.it/ec-oasis.owl#hasFee"/>
        <rdfs:domain rdf:resource="http://www.dmi.unict.it/ec-oasis.owl#SupplyChainPaymentPlan"/>
        <rdfs:range rdf:resource="http://www.dmi.unict.it/ec-oasis.owl#Fee"/>
        <rdfs:comment xml:lang="eng">This property connects a payment plan of supply chain with the related fee costs</rdfs:comment>
        <rdfs:label xml:lang="eng">has Payment Fee</rdfs:label>
    </owl:ObjectProperty>
    


    <!-- http://www.dmi.unict.it/ec-oasis.owl#hasPrice -->

    <owl:ObjectProperty rdf:about="http://www.dmi.unict.it/ec-oasis.owl#hasPrice">
        <rdfs:subPropertyOf rdf:resource="http://www.dmi.unict.it/oasis.owl#hasFeature"/>
        <rdfs:domain rdf:resource="http://www.dmi.unict.it/ec-oasis.owl#CommercialIssue"/>
        <rdfs:range rdf:resource="http://www.dmi.unict.it/ec-oasis.owl#Price"/>
        <rdfs:comment xml:lang="eng">This property connects an offering with the associated price</rdfs:comment>
        <rdfs:label xml:lang="eng">has Price</rdfs:label>
    </owl:ObjectProperty>
    


    <!-- http://www.dmi.unict.it/ec-oasis.owl#hasPriceDetail -->

    <owl:ObjectProperty rdf:about="http://www.dmi.unict.it/ec-oasis.owl#hasPriceDetail">
        <rdfs:subPropertyOf rdf:resource="http://www.dmi.unict.it/ec-oasis.owl#isOfferingPriceDescribedBy"/>
        <rdfs:subPropertyOf rdf:resource="http://www.dmi.unict.it/oasis.owl#hasCost"/>
        <rdfs:domain rdf:resource="http://www.dmi.unict.it/ec-oasis.owl#OfferingPrice"/>
        <rdfs:range rdf:resource="http://www.dmi.unict.it/oasis.owl#Cost"/>
        <rdfs:comment xml:lang="eng">This property connects the price of an offering the related monetary cost</rdfs:comment>
        <rdfs:label xml:lang="eng">has Price Detail</rdfs:label>
    </owl:ObjectProperty>
    


    <!-- http://www.dmi.unict.it/ec-oasis.owl#hasProofFee -->

    <owl:ObjectProperty rdf:about="http://www.dmi.unict.it/ec-oasis.owl#hasProofFee">
        <rdfs:subPropertyOf rdf:resource="http://www.dmi.unict.it/ec-oasis.owl#hasFee"/>
        <rdfs:domain rdf:resource="http://www.dmi.unict.it/ec-oasis.owl#SupplyChainProofPlan"/>
        <rdfs:range rdf:resource="http://www.dmi.unict.it/ec-oasis.owl#Fee"/>
        <rdfs:comment xml:lang="eng">This property connects a proof plan of supply chain with the related fee costs</rdfs:comment>
        <rdfs:label xml:lang="eng">has Proof Fee</rdfs:label>
    </owl:ObjectProperty>
    


    <!-- http://www.dmi.unict.it/ec-oasis.owl#hasPublisher -->

    <owl:ObjectProperty rdf:about="http://www.dmi.unict.it/ec-oasis.owl#hasPublisher">
        <rdfs:subPropertyOf rdf:resource="http://www.dmi.unict.it/oasis.owl#involves"/>
        <rdfs:domain rdf:resource="http://www.dmi.unict.it/ec-oasis.owl#OfferingPublishingActivity"/>
        <rdfs:range>
            <owl:Class>
                <owl:intersectionOf rdf:parseType="Collection">
                    <rdf:Description rdf:about="http://www.dmi.unict.it/oasis.owl#Agent"/>
                    <owl:Restriction>
                        <owl:onProperty rdf:resource="http://www.dmi.unict.it/oasis.owl#hasRole"/>
                        <owl:someValuesFrom rdf:resource="http://www.dmi.unict.it/ec-oasis.owl#Publisher"/>
                    </owl:Restriction>
                </owl:intersectionOf>
            </owl:Class>
        </rdfs:range>
        <rdfs:comment xml:lang="eng">This property connects an offering publishing activity with the publisher agent</rdfs:comment>
        <rdfs:label xml:lang="eng">has Publisher</rdfs:label>
    </owl:ObjectProperty>
    


    <!-- http://www.dmi.unict.it/ec-oasis.owl#hasPurchasableQuantity -->

    <owl:ObjectProperty rdf:about="http://www.dmi.unict.it/ec-oasis.owl#hasPurchasableQuantity">
        <rdfs:subPropertyOf rdf:resource="http://www.dmi.unict.it/ec-oasis.owl#isAvailabilityFeatureDescribedBy"/>
        <rdfs:subPropertyOf rdf:resource="http://www.dmi.unict.it/oasis.owl#hasQuantity"/>
        <rdfs:domain rdf:resource="http://www.dmi.unict.it/ec-oasis.owl#OfferingAvailability"/>
        <rdfs:range rdf:resource="http://www.dmi.unict.it/oasis.owl#Quantity"/>
        <rdfs:comment xml:lang="eng">This property connects an offering with the associated purchasable quantity feature</rdfs:comment>
        <rdfs:label xml:lang="eng">has Purchasable Quantity</rdfs:label>
    </owl:ObjectProperty>
    


    <!-- http://www.dmi.unict.it/ec-oasis.owl#hasQuantityAvailable -->

    <owl:ObjectProperty rdf:about="http://www.dmi.unict.it/ec-oasis.owl#hasQuantityAvailable">
        <rdfs:subPropertyOf rdf:resource="http://www.dmi.unict.it/ec-oasis.owl#isAvailabilityFeatureDescribedBy"/>
        <rdfs:subPropertyOf rdf:resource="http://www.dmi.unict.it/oasis.owl#hasQuantity"/>
        <rdfs:domain rdf:resource="http://www.dmi.unict.it/ec-oasis.owl#OfferingAvailability"/>
        <rdfs:range rdf:resource="http://www.dmi.unict.it/oasis.owl#Quantity"/>
        <rdfs:comment xml:lang="eng">This property connects an offering with the associated quantity availability feature</rdfs:comment>
        <rdfs:label xml:lang="eng">has Quantity Available</rdfs:label>
    </owl:ObjectProperty>
    


    <!-- http://www.dmi.unict.it/ec-oasis.owl#hasSeller -->

    <owl:ObjectProperty rdf:about="http://www.dmi.unict.it/ec-oasis.owl#hasSeller">
        <rdfs:subPropertyOf rdf:resource="http://www.dmi.unict.it/oasis.owl#involves"/>
        <rdfs:domain rdf:resource="http://www.dmi.unict.it/ec-oasis.owl#OfferingPublishingActivity"/>
        <rdfs:range>
            <owl:Class>
                <owl:intersectionOf rdf:parseType="Collection">
                    <rdf:Description rdf:about="http://www.dmi.unict.it/oasis.owl#Agent"/>
                    <owl:Restriction>
                        <owl:onProperty rdf:resource="http://www.dmi.unict.it/oasis.owl#hasRole"/>
                        <owl:someValuesFrom rdf:resource="http://www.dmi.unict.it/ec-oasis.owl#Seller"/>
                    </owl:Restriction>
                </owl:intersectionOf>
            </owl:Class>
        </rdfs:range>
        <rdfs:comment xml:lang="eng">This property connects an offering publishing activity with the seller agent</rdfs:comment>
        <rdfs:label xml:lang="eng">has Seller</rdfs:label>
    </owl:ObjectProperty>
    


    <!-- http://www.dmi.unict.it/ec-oasis.owl#hasSupplyChain -->

    <owl:ObjectProperty rdf:about="http://www.dmi.unict.it/ec-oasis.owl#hasSupplyChain">
        <rdfs:subPropertyOf rdf:resource="http://www.dmi.unict.it/oasis.owl#involves"/>
        <rdfs:domain rdf:resource="http://www.dmi.unict.it/ec-oasis.owl#CommercialIssue"/>
        <rdfs:range rdf:resource="http://www.dmi.unict.it/ec-oasis.owl#SupplyChain"/>
        <rdfs:comment xml:lang="eng">This property connects an offering  with the related supply chain</rdfs:comment>
        <rdfs:label xml:lang="eng">has Supply Chain</rdfs:label>
    </owl:ObjectProperty>
    


    <!-- http://www.dmi.unict.it/ec-oasis.owl#hasTaxFee -->

    <owl:ObjectProperty rdf:about="http://www.dmi.unict.it/ec-oasis.owl#hasTaxFee">
        <rdfs:subPropertyOf rdf:resource="http://www.dmi.unict.it/ec-oasis.owl#hasFee"/>
        <rdfs:subPropertyOf rdf:resource="http://www.dmi.unict.it/ec-oasis.owl#isOfferingPriceDescribedBy"/>
        <rdfs:domain rdf:resource="http://www.dmi.unict.it/ec-oasis.owl#OfferingPrice"/>
        <rdfs:range rdf:resource="http://www.dmi.unict.it/ec-oasis.owl#Fee"/>
        <rdfs:comment xml:lang="eng">This property connects an offering price with the related taxation cost</rdfs:comment>
        <rdfs:label xml:lang="eng">has Tax Fee</rdfs:label>
    </owl:ObjectProperty>
    


    <!-- http://www.dmi.unict.it/ec-oasis.owl#isAssetInExchange -->

    <owl:ObjectProperty rdf:about="http://www.dmi.unict.it/ec-oasis.owl#isAssetInExchange">
        <rdfs:subPropertyOf rdf:resource="http://www.dmi.unict.it/oasis.owl#involves"/>
        <rdfs:domain rdf:resource="http://www.dmi.unict.it/ec-oasis.owl#OfferingPrice"/>
        <rdfs:range rdf:resource="http://www.dmi.unict.it/oasis.owl#Asset"/>
        <rdfs:comment xml:lang="eng">This property connects the price of offerings with the asset that is given in exchange. It does not reguard only barter offering.</rdfs:comment>
        <rdfs:label xml:lang="eng">is Asset in Exchange</rdfs:label>
    </owl:ObjectProperty>
    


    <!-- http://www.dmi.unict.it/ec-oasis.owl#isAvailabilityFeatureDescribedBy -->

    <owl:ObjectProperty rdf:about="http://www.dmi.unict.it/ec-oasis.owl#isAvailabilityFeatureDescribedBy">
        <rdfs:subPropertyOf rdf:resource="http://www.dmi.unict.it/oasis.owl#isDescribedBy"/>
        <rdfs:domain rdf:resource="http://www.dmi.unict.it/ec-oasis.owl#OfferingAvailability"/>
        <rdfs:comment xml:lang="eng">This property connects an availability feature with the elements describing it</rdfs:comment>
        <rdfs:label xml:lang="eng">is Availability Feature Described By</rdfs:label>
    </owl:ObjectProperty>
    


    <!-- http://www.dmi.unict.it/ec-oasis.owl#isNegotiatedOn -->

    <owl:ObjectProperty rdf:about="http://www.dmi.unict.it/ec-oasis.owl#isNegotiatedOn">
        <rdfs:subPropertyOf rdf:resource="http://www.dmi.unict.it/oasis.owl#isRelatedWith"/>
        <rdf:type rdf:resource="http://www.w3.org/2002/07/owl#FunctionalProperty"/>
        <rdfs:domain rdf:resource="http://www.dmi.unict.it/ec-oasis.owl#NegotiationActivity"/>
        <rdfs:range rdf:resource="http://www.dmi.unict.it/ec-oasis.owl#CommercialIssue"/>
        <rdfs:comment xml:lang="eng">This property connects a negotiation activity with the offering for which the negotiation is proposed</rdfs:comment>
        <rdfs:label xml:lang="eng">is Negotiated On</rdfs:label>
    </owl:ObjectProperty>
    


    <!-- http://www.dmi.unict.it/ec-oasis.owl#isNegotiationFinalizedIn -->

    <owl:ObjectProperty rdf:about="http://www.dmi.unict.it/ec-oasis.owl#isNegotiationFinalizedIn">
        <rdfs:subPropertyOf rdf:resource="http://www.dmi.unict.it/oasis.owl#evolvesIn"/>
        <rdf:type rdf:resource="http://www.w3.org/2002/07/owl#FunctionalProperty"/>
        <rdfs:domain rdf:resource="http://www.dmi.unict.it/ec-oasis.owl#NegotiationActivity"/>
        <rdfs:range rdf:resource="http://www.dmi.unict.it/ec-oasis.owl#PurchaseActivity"/>
        <rdfs:comment xml:lang="eng">This property connects a successful negotiation with the final purchase activity</rdfs:comment>
        <rdfs:label xml:lang="eng">is Negotiation Finalized In</rdfs:label>
    </owl:ObjectProperty>
    


    <!-- http://www.dmi.unict.it/ec-oasis.owl#isOfferingAbout -->

    <owl:ObjectProperty rdf:about="http://www.dmi.unict.it/ec-oasis.owl#isOfferingAbout">
        <rdfs:subPropertyOf rdf:resource="http://www.dmi.unict.it/oasis.owl#involves"/>
        <rdfs:domain rdf:resource="http://www.dmi.unict.it/ec-oasis.owl#CommercialIssue"/>
        <rdfs:range rdf:resource="http://www.dmi.unict.it/oasis.owl#Asset"/>
        <rdfs:comment xml:lang="eng">This property connects an offering with the asset target of the offering</rdfs:comment>
        <rdfs:label xml:lang="eng">is Offering About</rdfs:label>
    </owl:ObjectProperty>
    


    <!-- http://www.dmi.unict.it/ec-oasis.owl#isOfferingPriceDescribedBy -->

    <owl:ObjectProperty rdf:about="http://www.dmi.unict.it/ec-oasis.owl#isOfferingPriceDescribedBy">
        <rdfs:subPropertyOf rdf:resource="http://www.dmi.unict.it/oasis.owl#isDescribedBy"/>
        <rdfs:domain rdf:resource="http://www.dmi.unict.it/ec-oasis.owl#OfferingPrice"/>
        <rdfs:comment xml:lang="eng">This property connects the offering price with the elements describing it</rdfs:comment>
        <rdfs:label xml:lang="eng">is Offering Price Described By</rdfs:label>
    </owl:ObjectProperty>
    


    <!-- http://www.dmi.unict.it/ec-oasis.owl#isPublishingAbout -->

    <owl:ObjectProperty rdf:about="http://www.dmi.unict.it/ec-oasis.owl#isPublishingAbout">
        <rdfs:subPropertyOf rdf:resource="http://www.dmi.unict.it/oasis.owl#involves"/>
        <rdf:type rdf:resource="http://www.w3.org/2002/07/owl#FunctionalProperty"/>
        <rdf:type rdf:resource="http://www.w3.org/2002/07/owl#InverseFunctionalProperty"/>
        <rdfs:domain rdf:resource="http://www.dmi.unict.it/ec-oasis.owl#OfferingPublishingActivity"/>
        <rdfs:range rdf:resource="http://www.dmi.unict.it/ec-oasis.owl#Offering"/>
        <rdfs:comment xml:lang="eng">This property connects an offering publishing activity with the published offering</rdfs:comment>
        <rdfs:label xml:lang="eng">is Publishing About</rdfs:label>
    </owl:ObjectProperty>
    


    <!-- http://www.dmi.unict.it/ec-oasis.owl#isPurchaseAbout -->

    <owl:ObjectProperty rdf:about="http://www.dmi.unict.it/ec-oasis.owl#isPurchaseAbout">
        <rdfs:subPropertyOf rdf:resource="http://www.dmi.unict.it/oasis.owl#involves"/>
        <rdfs:domain rdf:resource="http://www.dmi.unict.it/ec-oasis.owl#PurchaseActivity"/>
        <rdfs:range rdf:resource="http://www.w3.org/2002/07/owl#Thing"/>
        <rdfs:comment xml:lang="eng">This property connects an purchase activity with the acquired product</rdfs:comment>
        <rdfs:label xml:lang="eng">is Purchase About</rdfs:label>
    </owl:ObjectProperty>
    


    <!-- http://www.dmi.unict.it/ec-oasis.owl#negotiatesAbout -->

    <owl:ObjectProperty rdf:about="http://www.dmi.unict.it/ec-oasis.owl#negotiatesAbout">
        <rdfs:subPropertyOf rdf:resource="http://www.dmi.unict.it/oasis.owl#isRelatedWith"/>
        <rdfs:domain rdf:resource="http://www.dmi.unict.it/ec-oasis.owl#NegotiationActivity"/>
        <rdfs:range rdf:resource="http://www.dmi.unict.it/ec-oasis.owl#NegotiationOffering"/>
        <rdfs:comment xml:lang="eng">This property connects a negotiation activity with the object representing the nature of the negotiation</rdfs:comment>
        <rdfs:label xml:lang="eng">negotiates About</rdfs:label>
    </owl:ObjectProperty>
    


    <!-- http://www.dmi.unict.it/ec-oasis.owl#negotiationAcceptedBy -->

    <owl:ObjectProperty rdf:about="http://www.dmi.unict.it/ec-oasis.owl#negotiationAcceptedBy">
        <rdfs:subPropertyOf rdf:resource="http://www.dmi.unict.it/oasis.owl#involves"/>
        <rdfs:domain rdf:resource="http://www.dmi.unict.it/ec-oasis.owl#NegotiationActivity"/>
        <rdfs:range>
            <owl:Class>
                <owl:intersectionOf rdf:parseType="Collection">
                    <rdf:Description rdf:about="http://www.dmi.unict.it/oasis.owl#Agent"/>
                    <owl:Restriction>
                        <owl:onProperty rdf:resource="http://www.dmi.unict.it/oasis.owl#hasRole"/>
                        <owl:someValuesFrom>
                            <owl:Class>
                                <owl:unionOf rdf:parseType="Collection">
                                    <rdf:Description rdf:about="http://www.dmi.unict.it/ec-oasis.owl#Buyer"/>
                                    <rdf:Description rdf:about="http://www.dmi.unict.it/ec-oasis.owl#Seller"/>
                                </owl:unionOf>
                            </owl:Class>
                        </owl:someValuesFrom>
                    </owl:Restriction>
                </owl:intersectionOf>
            </owl:Class>
        </rdfs:range>
        <rdfs:comment xml:lang="eng">This property connects a negotiation activity with the buyer or seller that accepted it</rdfs:comment>
        <rdfs:label xml:lang="eng">negotiation Accepted By</rdfs:label>
    </owl:ObjectProperty>
    


    <!-- http://www.dmi.unict.it/ec-oasis.owl#negotiationPerformedBy -->

    <owl:ObjectProperty rdf:about="http://www.dmi.unict.it/ec-oasis.owl#negotiationPerformedBy">
        <rdfs:subPropertyOf rdf:resource="http://www.dmi.unict.it/oasis.owl#involves"/>
        <rdfs:domain rdf:resource="http://www.dmi.unict.it/ec-oasis.owl#NegotiationActivity"/>
        <rdfs:range>
            <owl:Class>
                <owl:intersectionOf rdf:parseType="Collection">
                    <rdf:Description rdf:about="http://www.dmi.unict.it/oasis.owl#Agent"/>
                    <owl:Restriction>
                        <owl:onProperty rdf:resource="http://www.dmi.unict.it/oasis.owl#hasRole"/>
                        <owl:someValuesFrom>
                            <owl:Class>
                                <owl:unionOf rdf:parseType="Collection">
                                    <rdf:Description rdf:about="http://www.dmi.unict.it/ec-oasis.owl#Buyer"/>
                                    <rdf:Description rdf:about="http://www.dmi.unict.it/ec-oasis.owl#Seller"/>
                                </owl:unionOf>
                            </owl:Class>
                        </owl:someValuesFrom>
                    </owl:Restriction>
                </owl:intersectionOf>
            </owl:Class>
        </rdfs:range>
        <rdfs:comment xml:lang="eng">This property connects a negotiation activity with the buyer or seller that proposed it</rdfs:comment>
        <rdfs:label xml:lang="eng">negotioation Performed By</rdfs:label>
    </owl:ObjectProperty>
    


    <!-- http://www.dmi.unict.it/ec-oasis.owl#negotiationRejectedBy -->

    <owl:ObjectProperty rdf:about="http://www.dmi.unict.it/ec-oasis.owl#negotiationRejectedBy">
        <rdfs:subPropertyOf rdf:resource="http://www.dmi.unict.it/oasis.owl#involves"/>
        <rdfs:domain rdf:resource="http://www.dmi.unict.it/ec-oasis.owl#NegotiationActivity"/>
        <rdfs:range>
            <owl:Class>
                <owl:intersectionOf rdf:parseType="Collection">
                    <rdf:Description rdf:about="http://www.dmi.unict.it/oasis.owl#Agent"/>
                    <owl:Restriction>
                        <owl:onProperty rdf:resource="http://www.dmi.unict.it/oasis.owl#hasRole"/>
                        <owl:someValuesFrom>
                            <owl:Class>
                                <owl:unionOf rdf:parseType="Collection">
                                    <rdf:Description rdf:about="http://www.dmi.unict.it/ec-oasis.owl#Buyer"/>
                                    <rdf:Description rdf:about="http://www.dmi.unict.it/ec-oasis.owl#Seller"/>
                                </owl:unionOf>
                            </owl:Class>
                        </owl:someValuesFrom>
                    </owl:Restriction>
                </owl:intersectionOf>
            </owl:Class>
        </rdfs:range>
        <rdfs:comment xml:lang="eng">This property connects a negotiation activity with the buyer or seller that rejected it</rdfs:comment>
        <rdfs:label xml:lang="eng">negotiation Rejected By</rdfs:label>
    </owl:ObjectProperty>
    


    <!-- http://www.dmi.unict.it/ec-oasis.owl#supplyChainImplementedBy -->

    <owl:ObjectProperty rdf:about="http://www.dmi.unict.it/ec-oasis.owl#supplyChainImplementedBy">
        <rdfs:subPropertyOf rdf:resource="http://www.dmi.unict.it/oasis.owl#implementedBy"/>
        <rdfs:domain rdf:resource="http://www.dmi.unict.it/ec-oasis.owl#SupplyChain"/>
        <rdfs:range rdf:resource="http://www.dmi.unict.it/ec-oasis.owl#SupplyChainPlan"/>
        <rdfs:comment xml:lang="eng">This property connects a supply chain with the plans that implement it</rdfs:comment>
        <rdfs:label xml:lang="eng">supply Chain Implemented By</rdfs:label>
    </owl:ObjectProperty>
    


    <!-- http://www.dmi.unict.it/oasis.owl#evolvesIn -->

    <owl:ObjectProperty rdf:about="http://www.dmi.unict.it/oasis.owl#evolvesIn"/>
    


    <!-- http://www.dmi.unict.it/oasis.owl#hasCost -->

    <owl:ObjectProperty rdf:about="http://www.dmi.unict.it/oasis.owl#hasCost"/>
    


    <!-- http://www.dmi.unict.it/oasis.owl#hasFeature -->

    <owl:ObjectProperty rdf:about="http://www.dmi.unict.it/oasis.owl#hasFeature"/>
    


    <!-- http://www.dmi.unict.it/oasis.owl#hasSpaceSpan -->

    <owl:ObjectProperty rdf:about="http://www.dmi.unict.it/oasis.owl#hasSpaceSpan"/>
    


    <!-- http://www.dmi.unict.it/oasis.owl#hasTimeSpan -->

    <owl:ObjectProperty rdf:about="http://www.dmi.unict.it/oasis.owl#hasTimeSpan"/>
    


    <!-- http://www.dmi.unict.it/oasis.owl#implementedBy -->

    <owl:ObjectProperty rdf:about="http://www.dmi.unict.it/oasis.owl#implementedBy"/>
    


    <!-- http://www.dmi.unict.it/oasis.owl#involves -->

    <owl:ObjectProperty rdf:about="http://www.dmi.unict.it/oasis.owl#involves"/>
    


    <!-- http://www.dmi.unict.it/oasis.owl#isDescribedBy -->

    <owl:ObjectProperty rdf:about="http://www.dmi.unict.it/oasis.owl#isDescribedBy"/>
    


    <!-- http://www.dmi.unict.it/oasis.owl#isRelatedWith -->

    <owl:ObjectProperty rdf:about="http://www.dmi.unict.it/oasis.owl#isRelatedWith"/>
    


    <!-- 
    ///////////////////////////////////////////////////////////////////////////////////////
    //
    // Data properties
    //
    ///////////////////////////////////////////////////////////////////////////////////////
     -->

    


    <!-- http://www.dmi.unict.it/ec-oasis.owl#hasCommercialIssueInformation -->

    <owl:DatatypeProperty rdf:about="http://www.dmi.unict.it/ec-oasis.owl#hasCommercialIssueInformation">
        <rdfs:subPropertyOf rdf:resource="http://www.dmi.unict.it/oasis.owl#hasDataValue"/>
    </owl:DatatypeProperty>
    


    <!-- http://www.dmi.unict.it/ec-oasis.owl#hasDescription -->

    <owl:DatatypeProperty rdf:about="http://www.dmi.unict.it/ec-oasis.owl#hasDescription">
        <rdfs:subPropertyOf rdf:resource="http://www.dmi.unict.it/ec-oasis.owl#hasCommercialIssueInformation"/>
        <rdfs:domain rdf:resource="http://www.dmi.unict.it/ec-oasis.owl#CommercialIssue"/>
        <rdfs:range rdf:resource="http://www.w3.org/2001/XMLSchema#string"/>
    </owl:DatatypeProperty>
    


    <!-- http://www.dmi.unict.it/ec-oasis.owl#hasID -->

    <owl:DatatypeProperty rdf:about="http://www.dmi.unict.it/ec-oasis.owl#hasID">
        <rdfs:subPropertyOf rdf:resource="http://www.dmi.unict.it/ec-oasis.owl#hasCommercialIssueInformation"/>
        <rdf:type rdf:resource="http://www.w3.org/2002/07/owl#FunctionalProperty"/>
        <rdfs:domain rdf:resource="http://www.dmi.unict.it/ec-oasis.owl#CommercialIssue"/>
        <rdfs:range rdf:resource="http://www.w3.org/2001/XMLSchema#string"/>
    </owl:DatatypeProperty>
    


    <!-- http://www.dmi.unict.it/oasis.owl#hasDataValue -->

    <owl:DatatypeProperty rdf:about="http://www.dmi.unict.it/oasis.owl#hasDataValue"/>
    


    <!-- 
    ///////////////////////////////////////////////////////////////////////////////////////
    //
    // Classes
    //
    ///////////////////////////////////////////////////////////////////////////////////////
     -->

    


    <!-- http://www.dmi.unict.it/ec-oasis.owl#AcceptedOffering -->

    <owl:Class rdf:about="http://www.dmi.unict.it/ec-oasis.owl#AcceptedOffering">
        <rdfs:subClassOf rdf:resource="http://www.dmi.unict.it/ec-oasis.owl#NegotiationOffering"/>
        <rdfs:comment xml:lang="eng">This class describes negotiations on offerings accepted as they are</rdfs:comment>
        <rdfs:label xml:lang="eng">Accepted Offering</rdfs:label>
    </owl:Class>
    


    <!-- http://www.dmi.unict.it/ec-oasis.owl#Auction -->

    <owl:Class rdf:about="http://www.dmi.unict.it/ec-oasis.owl#Auction">
        <rdfs:subClassOf rdf:resource="http://www.dmi.unict.it/ec-oasis.owl#Offering"/>
        <rdfs:comment xml:lang="eng">This class describes auctions</rdfs:comment>
        <rdfs:label xml:lang="eng">Auction</rdfs:label>
    </owl:Class>
    


    <!-- http://www.dmi.unict.it/ec-oasis.owl#AuctionBasePrice -->

    <owl:Class rdf:about="http://www.dmi.unict.it/ec-oasis.owl#AuctionBasePrice">
        <rdfs:subClassOf rdf:resource="http://www.dmi.unict.it/ec-oasis.owl#CommercialPerdurantFeature"/>
        <rdfs:subClassOf rdf:resource="http://www.dmi.unict.it/ec-oasis.owl#Price"/>
        <rdfs:label xml:lang="eng">Auction Base Price</rdfs:label>
        <rdfs:label xml:lang="eng">This class describes the starting price of auctions</rdfs:label>
    </owl:Class>
    


    <!-- http://www.dmi.unict.it/ec-oasis.owl#BarterOffering -->

    <owl:Class rdf:about="http://www.dmi.unict.it/ec-oasis.owl#BarterOffering">
        <rdfs:subClassOf rdf:resource="http://www.dmi.unict.it/ec-oasis.owl#Offering"/>
        <rdfs:comment xml:lang="eng">This class describes barters</rdfs:comment>
        <rdfs:label xml:lang="eng">Barter</rdfs:label>
    </owl:Class>
    


    <!-- http://www.dmi.unict.it/ec-oasis.owl#BatchSplitModificationActivity -->

    <owl:Class rdf:about="http://www.dmi.unict.it/ec-oasis.owl#BatchSplitModificationActivity">
        <rdfs:subClassOf rdf:resource="http://www.dmi.unict.it/oasis.owl#ModificationActivity"/>
        <rdfs:comment xml:lang="eng">This class describes modification activity carried on to split batches in smaller one(s)</rdfs:comment>
    </owl:Class>
    


    <!-- http://www.dmi.unict.it/ec-oasis.owl#Buyer -->

    <owl:Class rdf:about="http://www.dmi.unict.it/ec-oasis.owl#Buyer">
        <rdfs:subClassOf rdf:resource="http://www.dmi.unict.it/ec-oasis.owl#CommercialRole"/>
        <rdfs:comment xml:lang="eng">This class describes the role played by buyers in commercial activities</rdfs:comment>
        <rdfs:label xml:lang="eng">Buyer</rdfs:label>
    </owl:Class>
    


    <!-- http://www.dmi.unict.it/ec-oasis.owl#CommercialActivity -->

    <owl:Class rdf:about="http://www.dmi.unict.it/ec-oasis.owl#CommercialActivity">
        <rdfs:subClassOf rdf:resource="http://www.dmi.unict.it/oasis.owl#Activity"/>
        <rdfs:label xml:lang="eng">Commercial Activity</rdfs:label>
        <rdfs:label xml:lang="eng">This class describes commercial activities</rdfs:label>
    </owl:Class>
    


    <!-- http://www.dmi.unict.it/ec-oasis.owl#CommercialDescriptionObject -->

    <owl:Class rdf:about="http://www.dmi.unict.it/ec-oasis.owl#CommercialDescriptionObject">
        <rdfs:subClassOf rdf:resource="http://www.dmi.unict.it/oasis.owl#DescriptionObject"/>
        <rdfs:comment xml:lang="eng">This class comprises classes adopted as descriptional object for commercial stakeholders</rdfs:comment>
        <rdfs:label xml:lang="eng">Commercial Description Object</rdfs:label>
    </owl:Class>
    


    <!-- http://www.dmi.unict.it/ec-oasis.owl#CommercialIssue -->

    <owl:Class rdf:about="http://www.dmi.unict.it/ec-oasis.owl#CommercialIssue">
        <rdfs:subClassOf rdf:resource="http://www.dmi.unict.it/ec-oasis.owl#CommercialDescriptionObject"/>
        <rdfs:comment xml:lang="eng">This class comprises both offerings and their negotiations</rdfs:comment>
    </owl:Class>
    


    <!-- http://www.dmi.unict.it/ec-oasis.owl#CommercialPerdurantFeature -->

    <owl:Class rdf:about="http://www.dmi.unict.it/ec-oasis.owl#CommercialPerdurantFeature">
        <rdfs:subClassOf rdf:resource="http://www.dmi.unict.it/oasis.owl#PerdurantFeature"/>
        <rdfs:comment xml:lang="eng">This class describes perdurant features associated with offerings</rdfs:comment>
        <rdfs:label xml:lang="eng">Commercial Perdurant Feature</rdfs:label>
    </owl:Class>
    


    <!-- http://www.dmi.unict.it/ec-oasis.owl#CommercialRole -->

    <owl:Class rdf:about="http://www.dmi.unict.it/ec-oasis.owl#CommercialRole">
        <rdfs:subClassOf rdf:resource="http://www.dmi.unict.it/oasis.owl#Role"/>
        <rdfs:comment xml:lang="eng">This class describes commercial roles</rdfs:comment>
        <rdfs:label xml:lang="eng">Commercial Role</rdfs:label>
    </owl:Class>
    


    <!-- http://www.dmi.unict.it/ec-oasis.owl#ConditionedNegotiationActivity -->

    <owl:Class rdf:about="http://www.dmi.unict.it/ec-oasis.owl#ConditionedNegotiationActivity">
        <rdfs:subClassOf rdf:resource="http://www.dmi.unict.it/ec-oasis.owl#NegotiationActivity"/>
        <owl:disjointWith rdf:resource="http://www.dmi.unict.it/ec-oasis.owl#UnconditionedNegotiationActivity"/>
        <rdfs:comment xml:lang="eng">This class describes negotiations provided to reach a deal on offerings</rdfs:comment>
        <rdfs:label xml:lang="eng">Conditioned Negotiation Activity</rdfs:label>
    </owl:Class>
    


    <!-- http://www.dmi.unict.it/ec-oasis.owl#CounterOffering -->

    <owl:Class rdf:about="http://www.dmi.unict.it/ec-oasis.owl#CounterOffering">
        <rdfs:subClassOf rdf:resource="http://www.dmi.unict.it/ec-oasis.owl#NegotiationOffering"/>
        <rdfs:comment xml:lang="eng">This class describes counterofferings proposed by buyers in order to negotiate some conditions</rdfs:comment>
        <rdfs:label xml:lang="eng">CounterOffering</rdfs:label>
    </owl:Class>
    


    <!-- http://www.dmi.unict.it/ec-oasis.owl#CounterProposal -->

    <owl:Class rdf:about="http://www.dmi.unict.it/ec-oasis.owl#CounterProposal">
        <rdfs:subClassOf rdf:resource="http://www.dmi.unict.it/ec-oasis.owl#NegotiationOffering"/>
        <rdfs:comment xml:lang="eng">This class descibes counterproposal proposed by sellers as response to buyers counterofferings</rdfs:comment>
        <rdfs:label xml:lang="eng">Counterproposal</rdfs:label>
    </owl:Class>
    


    <!-- http://www.dmi.unict.it/ec-oasis.owl#Fee -->

    <owl:Class rdf:about="http://www.dmi.unict.it/ec-oasis.owl#Fee">
        <rdfs:subClassOf rdf:resource="http://www.dmi.unict.it/oasis.owl#Cost"/>
        <rdfs:comment xml:lang="eng">This class describes cost adopted as commercial fee on offering features</rdfs:comment>
        <rdfs:label xml:lang="eng">Fee</rdfs:label>
    </owl:Class>
    


    <!-- http://www.dmi.unict.it/ec-oasis.owl#LoanOffering -->

    <owl:Class rdf:about="http://www.dmi.unict.it/ec-oasis.owl#LoanOffering">
        <rdfs:subClassOf rdf:resource="http://www.dmi.unict.it/ec-oasis.owl#Offering"/>
        <rdfs:comment xml:lang="eng">This class describes loans</rdfs:comment>
        <rdfs:label xml:lang="eng">Loan Offering</rdfs:label>
    </owl:Class>
    


    <!-- http://www.dmi.unict.it/ec-oasis.owl#LocationEligibility -->

    <owl:Class rdf:about="http://www.dmi.unict.it/ec-oasis.owl#LocationEligibility">
        <rdfs:subClassOf rdf:resource="http://www.dmi.unict.it/ec-oasis.owl#CommercialPerdurantFeature"/>
        <rdfs:subClassOf rdf:resource="http://www.dmi.unict.it/ec-oasis.owl#NegotiableThing"/>
        <rdfs:comment xml:lang="eng">This class describes region eligibility features of offerings</rdfs:comment>
        <rdfs:label xml:lang="eng">Location Eligibility</rdfs:label>
    </owl:Class>
    


    <!-- http://www.dmi.unict.it/ec-oasis.owl#NegotiableThing -->

    <owl:Class rdf:about="http://www.dmi.unict.it/ec-oasis.owl#NegotiableThing">
        <rdfs:comment xml:lang="eng">Negotiable Thing</rdfs:comment>
        <rdfs:comment xml:lang="eng">This class describes things on which a negotiation can be carried on</rdfs:comment>
    </owl:Class>
    


    <!-- http://www.dmi.unict.it/ec-oasis.owl#NegotiationActivity -->

    <owl:Class rdf:about="http://www.dmi.unict.it/ec-oasis.owl#NegotiationActivity">
        <owl:equivalentClass>
            <owl:Class>
                <owl:unionOf rdf:parseType="Collection">
                    <rdf:Description rdf:about="http://www.dmi.unict.it/ec-oasis.owl#ConditionedNegotiationActivity"/>
                    <rdf:Description rdf:about="http://www.dmi.unict.it/ec-oasis.owl#UnconditionedNegotiationActivity"/>
                </owl:unionOf>
            </owl:Class>
        </owl:equivalentClass>
        <rdfs:subClassOf rdf:resource="http://www.dmi.unict.it/ec-oasis.owl#CommercialActivity"/>
        <rdfs:comment xml:lang="eng">This class describes negotiations carried on offerings</rdfs:comment>
        <rdfs:label xml:lang="eng">This class describes negotiations carried on offerings</rdfs:label>
    </owl:Class>
    


    <!-- http://www.dmi.unict.it/ec-oasis.owl#NegotiationOffering -->

    <owl:Class rdf:about="http://www.dmi.unict.it/ec-oasis.owl#NegotiationOffering">
        <rdfs:subClassOf rdf:resource="http://www.dmi.unict.it/ec-oasis.owl#CommercialIssue"/>
        <rdfs:comment xml:lang="eng">This class comprises negotiations carried on offerings</rdfs:comment>
        <rdfs:label xml:lang="eng">Negotiation Offering</rdfs:label>
    </owl:Class>
    


    <!-- http://www.dmi.unict.it/ec-oasis.owl#Offering -->

    <owl:Class rdf:about="http://www.dmi.unict.it/ec-oasis.owl#Offering">
        <rdfs:subClassOf rdf:resource="http://www.dmi.unict.it/ec-oasis.owl#CommercialIssue"/>
        <rdfs:comment xml:lang="eng">This class comprises commercial offerings</rdfs:comment>
        <rdfs:label xml:lang="eng">Offering</rdfs:label>
    </owl:Class>
    


    <!-- http://www.dmi.unict.it/ec-oasis.owl#OfferingAvailability -->

    <owl:Class rdf:about="http://www.dmi.unict.it/ec-oasis.owl#OfferingAvailability">
        <rdfs:subClassOf rdf:resource="http://www.dmi.unict.it/ec-oasis.owl#CommercialPerdurantFeature"/>
        <rdfs:subClassOf rdf:resource="http://www.dmi.unict.it/ec-oasis.owl#NegotiableThing"/>
        <rdfs:comment xml:lang="eng">This class describes availability features of offerings</rdfs:comment>
        <rdfs:label xml:lang="eng">Offering Availability</rdfs:label>
    </owl:Class>
    


    <!-- http://www.dmi.unict.it/ec-oasis.owl#OfferingPrice -->

    <owl:Class rdf:about="http://www.dmi.unict.it/ec-oasis.owl#OfferingPrice">
        <rdfs:subClassOf rdf:resource="http://www.dmi.unict.it/ec-oasis.owl#CommercialPerdurantFeature"/>
        <rdfs:subClassOf rdf:resource="http://www.dmi.unict.it/ec-oasis.owl#Price"/>
        <rdfs:comment xml:lang="eng">This class describes the price of an offering</rdfs:comment>
        <rdfs:label xml:lang="eng">Price</rdfs:label>
    </owl:Class>
    


    <!-- http://www.dmi.unict.it/ec-oasis.owl#OfferingPublishingActivity -->

    <owl:Class rdf:about="http://www.dmi.unict.it/ec-oasis.owl#OfferingPublishingActivity">
        <rdfs:subClassOf rdf:resource="http://www.dmi.unict.it/ec-oasis.owl#CommercialActivity"/>
        <rdfs:comment xml:lang="eng">This class describes the activity of publishing commercial offerings</rdfs:comment>
        <rdfs:label xml:lang="eng">Offering Publishing Activity</rdfs:label>
    </owl:Class>
    


    <!-- http://www.dmi.unict.it/ec-oasis.owl#PawnOffering -->

    <owl:Class rdf:about="http://www.dmi.unict.it/ec-oasis.owl#PawnOffering">
        <rdfs:subClassOf rdf:resource="http://www.dmi.unict.it/ec-oasis.owl#Offering"/>
        <rdfs:comment xml:lang="eng">This class describes pawns</rdfs:comment>
        <rdfs:label xml:lang="eng">Pawn Offering</rdfs:label>
    </owl:Class>
    


    <!-- http://www.dmi.unict.it/ec-oasis.owl#PaymentMethodType -->

    <owl:Class rdf:about="http://www.dmi.unict.it/ec-oasis.owl#PaymentMethodType">
        <rdfs:subClassOf rdf:resource="http://www.dmi.unict.it/ec-oasis.owl#CommercialDescriptionObject"/>
        <rdfs:comment xml:lang="eng">This class describes payment method types</rdfs:comment>
        <rdfs:label xml:lang="eng">Payment Method Type</rdfs:label>
    </owl:Class>
    


    <!-- http://www.dmi.unict.it/ec-oasis.owl#Price -->

    <owl:Class rdf:about="http://www.dmi.unict.it/ec-oasis.owl#Price">
        <rdfs:subClassOf rdf:resource="http://www.dmi.unict.it/ec-oasis.owl#NegotiableThing"/>
        <rdfs:comment xml:lang="eng">This class describes prices</rdfs:comment>
        <rdfs:label xml:lang="eng">Price</rdfs:label>
    </owl:Class>
    


    <!-- http://www.dmi.unict.it/ec-oasis.owl#Publisher -->

    <owl:Class rdf:about="http://www.dmi.unict.it/ec-oasis.owl#Publisher">
        <rdfs:subClassOf rdf:resource="http://www.dmi.unict.it/ec-oasis.owl#CommercialRole"/>
        <rdfs:comment xml:lang="eng">This class describes the role played by publishers in commercial activities</rdfs:comment>
        <rdfs:label xml:lang="eng">Publisher</rdfs:label>
    </owl:Class>
    


    <!-- http://www.dmi.unict.it/ec-oasis.owl#PurchaseActivity -->

    <owl:Class rdf:about="http://www.dmi.unict.it/ec-oasis.owl#PurchaseActivity">
        <rdfs:subClassOf rdf:resource="http://www.dmi.unict.it/ec-oasis.owl#CommercialActivity"/>
        <rdfs:comment xml:lang="eng">This class describes the purchase activity as final step of negotiations successifully ended.</rdfs:comment>
        <rdfs:label xml:lang="eng">Purchase Activity</rdfs:label>
    </owl:Class>
    


    <!-- http://www.dmi.unict.it/ec-oasis.owl#SellOffering -->

    <owl:Class rdf:about="http://www.dmi.unict.it/ec-oasis.owl#SellOffering">
        <rdfs:subClassOf rdf:resource="http://www.dmi.unict.it/ec-oasis.owl#Offering"/>
        <rdfs:comment xml:lang="eng">This class describes standard sell offerings</rdfs:comment>
        <rdfs:label xml:lang="eng">Sell Offering</rdfs:label>
    </owl:Class>
    


    <!-- http://www.dmi.unict.it/ec-oasis.owl#Seller -->

    <owl:Class rdf:about="http://www.dmi.unict.it/ec-oasis.owl#Seller">
        <rdfs:subClassOf rdf:resource="http://www.dmi.unict.it/ec-oasis.owl#CommercialRole"/>
        <rdfs:comment xml:lang="eng">This class describes the role played by sellers in commercial activities</rdfs:comment>
        <rdfs:label xml:lang="eng">Seller</rdfs:label>
    </owl:Class>
    


    <!-- http://www.dmi.unict.it/ec-oasis.owl#StockWithdrawalModificationActivity -->

    <owl:Class rdf:about="http://www.dmi.unict.it/ec-oasis.owl#StockWithdrawalModificationActivity">
        <rdfs:subClassOf rdf:resource="http://www.dmi.unict.it/oasis.owl#ModificationActivity"/>
        <rdfs:comment xml:lang="eng">This class describes modification activities carried on to take specimen from stocks for selling purposes</rdfs:comment>
    </owl:Class>
    


    <!-- http://www.dmi.unict.it/ec-oasis.owl#SupplyChain -->

    <owl:Class rdf:about="http://www.dmi.unict.it/ec-oasis.owl#SupplyChain">
        <rdfs:subClassOf rdf:resource="http://www.dmi.unict.it/ec-oasis.owl#CommercialActivity"/>
        <rdfs:subClassOf rdf:resource="http://www.dmi.unict.it/ec-oasis.owl#NegotiableThing"/>
        <rdfs:comment xml:lang="eng">This class describes supply chain associated with offerings</rdfs:comment>
        <rdfs:label xml:lang="eng">Supply Chain</rdfs:label>
    </owl:Class>
    


    <!-- http://www.dmi.unict.it/ec-oasis.owl#SupplyChainAcquisitionPlan -->

    <owl:Class rdf:about="http://www.dmi.unict.it/ec-oasis.owl#SupplyChainAcquisitionPlan">
        <rdfs:subClassOf rdf:resource="http://www.dmi.unict.it/ec-oasis.owl#SupplyChainPlan"/>
        <rdfs:comment xml:lang="eng">This class describes OASIS plan associated with the product acquisition indicated by offering supply chains</rdfs:comment>
        <rdfs:label xml:lang="eng">Supply Chain Acquisition Plan</rdfs:label>
    </owl:Class>
    


    <!-- http://www.dmi.unict.it/ec-oasis.owl#SupplyChainDeliveryPlan -->

    <owl:Class rdf:about="http://www.dmi.unict.it/ec-oasis.owl#SupplyChainDeliveryPlan">
        <rdfs:subClassOf rdf:resource="http://www.dmi.unict.it/ec-oasis.owl#SupplyChainAcquisitionPlan"/>
        <rdfs:comment xml:lang="eng">This class describes OASIS plan associated with the product delivery indicated by offering supply chains</rdfs:comment>
        <rdfs:label xml:lang="eng">Supply Chain Delivery Plan</rdfs:label>
    </owl:Class>
    


    <!-- http://www.dmi.unict.it/ec-oasis.owl#SupplyChainFunctionPlan -->

    <owl:Class rdf:about="http://www.dmi.unict.it/ec-oasis.owl#SupplyChainFunctionPlan">
        <rdfs:subClassOf rdf:resource="http://www.dmi.unict.it/ec-oasis.owl#SupplyChainPlan"/>
        <rdfs:comment xml:lang="eng">This class describes OASIS plan associated with the purpose of the offering indicated in the related supply chain</rdfs:comment>
        <rdfs:label xml:lang="eng">Supply Chain Function Plan</rdfs:label>
    </owl:Class>
    


    <!-- http://www.dmi.unict.it/ec-oasis.owl#SupplyChainPaymentPlan -->

    <owl:Class rdf:about="http://www.dmi.unict.it/ec-oasis.owl#SupplyChainPaymentPlan">
        <rdfs:subClassOf rdf:resource="http://www.dmi.unict.it/ec-oasis.owl#SupplyChainPlan"/>
        <rdfs:comment xml:lang="eng">This class describes OASIS plan associated with the product payment indicated by offering supply chains</rdfs:comment>
        <rdfs:label xml:lang="eng">Supply Chain Payment Plan</rdfs:label>
    </owl:Class>
    


    <!-- http://www.dmi.unict.it/ec-oasis.owl#SupplyChainPickUpPlan -->

    <owl:Class rdf:about="http://www.dmi.unict.it/ec-oasis.owl#SupplyChainPickUpPlan">
        <rdfs:subClassOf rdf:resource="http://www.dmi.unict.it/ec-oasis.owl#SupplyChainAcquisitionPlan"/>
        <rdfs:comment xml:lang="eng">This class describes OASIS plan associated with the local pick up of products indicated by offering supply chains</rdfs:comment>
        <rdfs:label xml:lang="eng">Supply Chain Pick Up Plan</rdfs:label>
    </owl:Class>
    


    <!-- http://www.dmi.unict.it/ec-oasis.owl#SupplyChainPlan -->

    <owl:Class rdf:about="http://www.dmi.unict.it/ec-oasis.owl#SupplyChainPlan">
        <rdfs:subClassOf rdf:resource="http://www.dmi.unict.it/oasis.owl#PlanDescription"/>
        <rdfs:comment xml:lang="eng">This class describes OASIS plan associated with the realization of offering supply chains</rdfs:comment>
        <rdfs:label xml:lang="eng">Supply Chain Plan</rdfs:label>
    </owl:Class>
    


    <!-- http://www.dmi.unict.it/ec-oasis.owl#SupplyChainProofPlan -->

    <owl:Class rdf:about="http://www.dmi.unict.it/ec-oasis.owl#SupplyChainProofPlan">
        <rdfs:subClassOf rdf:resource="http://www.dmi.unict.it/ec-oasis.owl#SupplyChainPlan"/>
        <rdfs:comment xml:lang="eng">This class describes OASIS plan associated with the release of proofs (such as receipts and tokens) indicated by offering supply chains</rdfs:comment>
        <rdfs:label xml:lang="eng">Supply Chain Proof Plan</rdfs:label>
    </owl:Class>
    


    <!-- http://www.dmi.unict.it/ec-oasis.owl#UnconditionedNegotiationActivity -->

    <owl:Class rdf:about="http://www.dmi.unict.it/ec-oasis.owl#UnconditionedNegotiationActivity">
        <rdfs:subClassOf rdf:resource="http://www.dmi.unict.it/ec-oasis.owl#NegotiationActivity"/>
        <rdfs:comment xml:lang="eng">This class describes negotiations provided to accept offerings as they are</rdfs:comment>
        <rdfs:label xml:lang="eng">Unconditioned Negotiation Activity</rdfs:label>
    </owl:Class>
    


    <!-- http://www.dmi.unict.it/oasis.owl#Activity -->

    <owl:Class rdf:about="http://www.dmi.unict.it/oasis.owl#Activity"/>
    


    <!-- http://www.dmi.unict.it/oasis.owl#Agent -->

    <owl:Class rdf:about="http://www.dmi.unict.it/oasis.owl#Agent"/>
    


    <!-- http://www.dmi.unict.it/oasis.owl#Asset -->

    <owl:Class rdf:about="http://www.dmi.unict.it/oasis.owl#Asset"/>
    


    <!-- http://www.dmi.unict.it/oasis.owl#Cost -->

    <owl:Class rdf:about="http://www.dmi.unict.it/oasis.owl#Cost"/>
    


    <!-- http://www.dmi.unict.it/oasis.owl#Currency -->

    <owl:Class rdf:about="http://www.dmi.unict.it/oasis.owl#Currency"/>
    


    <!-- http://www.dmi.unict.it/oasis.owl#DescriptionObject -->

    <owl:Class rdf:about="http://www.dmi.unict.it/oasis.owl#DescriptionObject"/>
    


    <!-- http://www.dmi.unict.it/oasis.owl#EndurantFeature -->

    <owl:Class rdf:about="http://www.dmi.unict.it/oasis.owl#EndurantFeature"/>
    


    <!-- http://www.dmi.unict.it/oasis.owl#Measurement -->

    <owl:Class rdf:about="http://www.dmi.unict.it/oasis.owl#Measurement"/>
    


    <!-- http://www.dmi.unict.it/oasis.owl#NumericCost -->

    <owl:Class rdf:about="http://www.dmi.unict.it/oasis.owl#NumericCost"/>
    


    <!-- http://www.dmi.unict.it/oasis.owl#PlanDescription -->

    <owl:Class rdf:about="http://www.dmi.unict.it/oasis.owl#PlanDescription"/>
    


    <!-- http://www.dmi.unict.it/oasis.owl#Space -->

    <owl:Class rdf:about="http://www.dmi.unict.it/oasis.owl#Space"/>
    


    <!-- http://www.dmi.unict.it/oasis.owl#TimeWindow -->

    <owl:Class rdf:about="http://www.dmi.unict.it/oasis.owl#TimeWindow"/>
</rdf:RDF>



<!-- Generated by the OWL API (version 4.5.9.2019-02-01T07:24:44Z) https://github.com/owlcs/owlapi -->

