<?xml version="1.0"?>
<rdf:RDF xmlns="http://www.ngi.ontochain/ontologies/oc-found.owl#"
     xml:base="http://www.ngi.ontochain/ontologies/oc-found.owl"
     xmlns:owl="http://www.w3.org/2002/07/owl#"
     xmlns:rdf="http://www.w3.org/1999/02/22-rdf-syntax-ns#"
     xmlns:xml="http://www.w3.org/XML/1998/namespace"
     xmlns:xsd="http://www.w3.org/2001/XMLSchema#"
     xmlns:rdfs="http://www.w3.org/2000/01/rdf-schema#"
     xmlns:oasis="http://www.dmi.unict.it/oasis.owl#"
     xmlns:terms="http://purl.org/dc/terms/">
    <owl:Ontology rdf:about="http://www.ngi.ontochain/ontologies/oc-found.owl">
        <owl:imports rdf:resource="http://www.dmi.unict.it/oasis-abox.owl"/>
        <owl:imports rdf:resource="http://www.dmi.unict.it/oasis.owl"/>
        <terms:created rdf:datatype="http://www.w3.org/2001/XMLSchema#string">Cristiano Longo</terms:created>
        <terms:created rdf:datatype="http://www.w3.org/2001/XMLSchema#string">Daniele Francesco Santamaria</terms:created>
        <terms:created rdf:datatype="http://www.w3.org/2001/XMLSchema#string">Domenico Cantone</terms:created>
        <terms:created rdf:datatype="http://www.w3.org/2001/XMLSchema#string">Giampaolo Bella</terms:created>
        <terms:created rdf:datatype="http://www.w3.org/2001/XMLSchema#string">Marianna Nicolosi Asmundo</terms:created>
        <terms:license>This program is free software: you can redistribute it and/or modify it under the terms of the GNU General Public License as published by the Free Software Foundation, either version 3 of the License, or (at your option) any later version. This program is distributed in the hope that it will be useful, but WITHOUT ANY WARRANTY; without even the implied warranty of MERCHANTABILITY or FITNESS FOR A PARTICULAR PURPOSE. See the GNU General Public License for more details. You should have received a copy of the GNU General Public License along with this program. If not, see http://www.gnu.org/licenses/.</terms:license>
    </owl:Ontology>
    


    <!-- 
    ///////////////////////////////////////////////////////////////////////////////////////
    //
    // Annotation properties
    //
    ///////////////////////////////////////////////////////////////////////////////////////
     -->

    


    <!-- http://purl.org/dc/terms/license -->

    <owl:AnnotationProperty rdf:about="http://purl.org/dc/terms/license"/>
    


    <!-- 
    ///////////////////////////////////////////////////////////////////////////////////////
    //
    // Object Properties
    //
    ///////////////////////////////////////////////////////////////////////////////////////
     -->

    


    <!-- http://www.ngi.ontochain/ontologies/oc-found.owl#hasDigitalIdentity -->

    <owl:ObjectProperty rdf:about="http://www.ngi.ontochain/ontologies/oc-found.owl#hasDigitalIdentity">
        <rdfs:subPropertyOf rdf:resource="http://www.dmi.unict.it/oasis.owl#owns"/>
        <rdfs:domain rdf:resource="http://www.dmi.unict.it/oasis.owl#Agent"/>
        <rdfs:range rdf:resource="http://www.ngi.ontochain/ontologies/oc-found.owl#DigitalIdentity"/>
        <rdfs:comment xml:lang="en">This property connects agents to their digital identities, i.e., instance of DigitalIdentity</rdfs:comment>
    </owl:ObjectProperty>
    


    <!-- http://www.ngi.ontochain/ontologies/oc-found.owl#hasQualityValuationResult -->

    <owl:ObjectProperty rdf:about="http://www.ngi.ontochain/ontologies/oc-found.owl#hasQualityValuationResult">
        <rdfs:subPropertyOf rdf:resource="http://www.dmi.unict.it/oasis.owl#hasCompositeValue"/>
        <rdfs:domain rdf:resource="http://www.ngi.ontochain/ontologies/oc-found.owl#QualityValuationActivity"/>
        <rdfs:range rdf:resource="http://www.ngi.ontochain/ontologies/oc-found.owl#QualityValuationResult"/>
        <rdfs:comment xml:lang="en">This property connects a quality valuation activity (i.e., instance of QualityValuationActivity) to quality valuation result computed</rdfs:comment>
    </owl:ObjectProperty>
    


    <!-- http://www.ngi.ontochain/ontologies/oc-found.owl#hasSupplyChainActivity -->

    <owl:ObjectProperty rdf:about="http://www.ngi.ontochain/ontologies/oc-found.owl#hasSupplyChainActivity">
        <rdfs:subPropertyOf rdf:resource="http://www.dmi.unict.it/oasis.owl#encompassesActivity"/>
        <rdfs:domain rdf:resource="http://www.ngi.ontochain/ontologies/oc-found.owl#SupplyChainManagement"/>
        <rdfs:range rdf:resource="http://www.ngi.ontochain/ontologies/oc-found.owl#SupplyChainActivity"/>
        <rdfs:comment xml:lang="en">This property connects a supply chain management activity to its internal activities</rdfs:comment>
    </owl:ObjectProperty>
    


    <!-- http://www.ngi.ontochain/ontologies/oc-found.owl#hasSupplyChainManagement -->

    <owl:ObjectProperty rdf:about="http://www.ngi.ontochain/ontologies/oc-found.owl#hasSupplyChainManagement">
        <rdfs:subPropertyOf rdf:resource="http://www.dmi.unict.it/oasis.owl#isRelatedWithActivity"/>
        <rdfs:range rdf:resource="http://www.ngi.ontochain/ontologies/oc-found.owl#SupplyChainManagement"/>
        <rdfs:comment xml:lang="en">This property connects a resource to its supply chain management activity</rdfs:comment>
    </owl:ObjectProperty>
    


    <!-- http://www.ngi.ontochain/ontologies/oc-found.owl#performsQualityValuation -->

    <owl:ObjectProperty rdf:about="http://www.ngi.ontochain/ontologies/oc-found.owl#performsQualityValuation">
        <rdfs:subPropertyOf rdf:resource="http://www.dmi.unict.it/oasis.owl#isRelatedWithActivity"/>
        <rdfs:subPropertyOf rdf:resource="http://www.dmi.unict.it/oasis.owl#performs"/>
        <rdfs:domain rdf:resource="http://www.ngi.ontochain/ontologies/oc-found.owl#QualityValuerAgent"/>
        <rdfs:range rdf:resource="http://www.ngi.ontochain/ontologies/oc-found.owl#QualityValuationActivity"/>
        <rdfs:comment xml:lang="en">This property connects a valuer agent (i.e., instance of QualityValuerAgent) to the performed quality valuation activity (i.e., instance of QualityValuationActivity)</rdfs:comment>
    </owl:ObjectProperty>
    


    <!-- http://www.ngi.ontochain/ontologies/oc-found.owl#qualityValuationPerformedOn -->

    <owl:ObjectProperty rdf:about="http://www.ngi.ontochain/ontologies/oc-found.owl#qualityValuationPerformedOn">
        <rdfs:subPropertyOf rdf:resource="http://www.dmi.unict.it/oasis.owl#involves"/>
        <rdfs:domain rdf:resource="http://www.ngi.ontochain/ontologies/oc-found.owl#QualityValuationActivity"/>
        <rdfs:comment xml:lang="en">This property connects a quality valuation activity (i.e., instance of QualityValuationActivity) to the resource for which the quality valuation has been performed</rdfs:comment>
    </owl:ObjectProperty>
    


    <!-- http://www.ngi.ontochain/ontologies/oc-found.owl#supplyChainActivityImplementedBy -->

    <owl:ObjectProperty rdf:about="http://www.ngi.ontochain/ontologies/oc-found.owl#supplyChainActivityImplementedBy">
        <rdfs:subPropertyOf rdf:resource="http://www.dmi.unict.it/oasis.owl#implementedBy"/>
        <rdfs:domain rdf:resource="http://www.ngi.ontochain/ontologies/oc-found.owl#SupplyChainActivity"/>
        <rdfs:range>
            <owl:Class>
                <owl:unionOf rdf:parseType="Collection">
                    <rdf:Description rdf:about="http://www.dmi.unict.it/oasis.owl#Asset"/>
                    <rdf:Description rdf:about="http://www.dmi.unict.it/oasis.owl#Behavior"/>
                </owl:unionOf>
            </owl:Class>
        </rdfs:range>
    </owl:ObjectProperty>
    


    <!-- 
    ///////////////////////////////////////////////////////////////////////////////////////
    //
    // Classes
    //
    ///////////////////////////////////////////////////////////////////////////////////////
     -->

    


    <!-- http://www.ngi.ontochain/ontologies/oc-found.owl#DigitalIdentity -->

    <owl:Class rdf:about="http://www.ngi.ontochain/ontologies/oc-found.owl#DigitalIdentity">
        <rdfs:subClassOf rdf:resource="http://www.dmi.unict.it/oasis.owl#DescriptionObject"/>
        <rdfs:comment xml:lang="en">This class describes the digital identities associated with legal entities or agents</rdfs:comment>
    </owl:Class>
    


    <!-- http://www.ngi.ontochain/ontologies/oc-found.owl#LegalEntity -->

    <owl:Class rdf:about="http://www.ngi.ontochain/ontologies/oc-found.owl#LegalEntity">
        <rdfs:subClassOf rdf:resource="http://www.dmi.unict.it/oasis.owl#Agent"/>
        <rdfs:comment xml:lang="en">This class describes legal entities such as companies, people, societies</rdfs:comment>
    </owl:Class>
    


    <!-- http://www.ngi.ontochain/ontologies/oc-found.owl#QualityValuationActivity -->

    <owl:Class rdf:about="http://www.ngi.ontochain/ontologies/oc-found.owl#QualityValuationActivity">
        <rdfs:subClassOf rdf:resource="http://www.dmi.unict.it/oasis.owl#Activity"/>
        <rdfs:comment xml:lang="en">This class describes a quality valuation activity performed by some quality valuer agents (i.e., instance of QualityValuerAgent)</rdfs:comment>
    </owl:Class>
    


    <!-- http://www.ngi.ontochain/ontologies/oc-found.owl#QualityValuationResult -->

    <owl:Class rdf:about="http://www.ngi.ontochain/ontologies/oc-found.owl#QualityValuationResult">
        <rdfs:subClassOf rdf:resource="http://www.dmi.unict.it/oasis.owl#CompositeValue"/>
        <rdfs:comment xml:lang="en">This class describes the output of a quality valuation performed by a quality valuer agent, i.e., instance of QualityValuerAgent</rdfs:comment>
    </owl:Class>
    


    <!-- http://www.ngi.ontochain/ontologies/oc-found.owl#QualityValuerAgent -->

    <owl:Class rdf:about="http://www.ngi.ontochain/ontologies/oc-found.owl#QualityValuerAgent">
        <rdfs:subClassOf rdf:resource="http://www.dmi.unict.it/oasis.owl#Agent"/>
        <rdfs:comment xml:lang="en">This class describes a quality valuer agent, i.e., an agent performing quality valuations on resources of supply chain activities.</rdfs:comment>
    </owl:Class>
    


    <!-- http://www.ngi.ontochain/ontologies/oc-found.owl#SupplyChainActivity -->

    <owl:Class rdf:about="http://www.ngi.ontochain/ontologies/oc-found.owl#SupplyChainActivity">
        <rdfs:subClassOf rdf:resource="http://www.ngi.ontochain/ontologies/oc-found.owl#SupplyChainThing"/>
        <rdfs:comment xml:lang="en">This class describes an activity concerning the supply chain of resources</rdfs:comment>
    </owl:Class>
    


    <!-- http://www.ngi.ontochain/ontologies/oc-found.owl#SupplyChainDeliveryActivity -->

    <owl:Class rdf:about="http://www.ngi.ontochain/ontologies/oc-found.owl#SupplyChainDeliveryActivity">
        <rdfs:subClassOf rdf:resource="http://www.ngi.ontochain/ontologies/oc-found.owl#SupplyChainActivity"/>
        <rdfs:comment xml:lang="en">This class describes the delivery activity  of resources involved in some supply chains.</rdfs:comment>
    </owl:Class>
    


    <!-- http://www.ngi.ontochain/ontologies/oc-found.owl#SupplyChainManagement -->

    <owl:Class rdf:about="http://www.ngi.ontochain/ontologies/oc-found.owl#SupplyChainManagement">
        <rdfs:subClassOf rdf:resource="http://www.ngi.ontochain/ontologies/oc-found.owl#SupplyChainThing"/>
        <rdfs:comment xml:lang="en">This class describes the management activity concerning supply chain of resources</rdfs:comment>
    </owl:Class>
    


    <!-- http://www.ngi.ontochain/ontologies/oc-found.owl#SupplyChainPaymentActivity -->

    <owl:Class rdf:about="http://www.ngi.ontochain/ontologies/oc-found.owl#SupplyChainPaymentActivity">
        <rdfs:subClassOf rdf:resource="http://www.ngi.ontochain/ontologies/oc-found.owl#SupplyChainActivity"/>
        <rdfs:comment xml:lang="en">This class describes the payment activity  of resources involved in some supply chains.</rdfs:comment>
    </owl:Class>
    


    <!-- http://www.ngi.ontochain/ontologies/oc-found.owl#SSupplyChainOfferingProofActivity -->

    <owl:Class rdf:about="http://www.ngi.ontochain/ontologies/oc-found.owl#SupplyChainOfferingProofActivity">
        <rdfs:subClassOf rdf:resource="http://www.ngi.ontochain/ontologies/oc-found.owl#SupplyChainActivity"/>
    </owl:Class>
    


    <!-- http://www.ngi.ontochain/ontologies/oc-found.owl#SupplyChainReleaseActivity -->

    <owl:Class rdf:about="http://www.ngi.ontochain/ontologies/oc-found.owl#SupplyChainReleaseActivity">
        <rdfs:subClassOf rdf:resource="http://www.ngi.ontochain/ontologies/oc-found.owl#SupplyChainActivity"/>
        <rdfs:comment xml:lang="en">This class describes the release activity  of resources involved in some supply chains.</rdfs:comment>
    </owl:Class>
    


    <!-- http://www.ngi.ontochain/ontologies/oc-found.owl#SupplyChainThing -->

    <owl:Class rdf:about="http://www.ngi.ontochain/ontologies/oc-found.owl#SupplyChainThing">
        <rdfs:subClassOf rdf:resource="http://www.dmi.unict.it/oasis.owl#Activity"/>
        <rdfs:comment xml:lang="en">This class  encompasses all the classes concerning the supply chain environment</rdfs:comment>
    </owl:Class>
</rdf:RDF>



<!-- Generated by the OWL API (version 4.5.9.2019-02-01T07:24:44Z) https://github.com/owlcs/owlapi -->

